secure_example/LabelledImpInlineTypesProgInsens.v
@@ -49,38 +49,36 @@ Local Open Scope string_scope.
 
 Section LabelledImpTypesProgInsens.
 
-Notation label := sensitivity.
+Context (Labels : Lattice).
+Context (HLabels : LatticeLaws Labels).
+Notation label := (@T Labels).
 
-Definition labelled_equiv  :=
-  LabelledImpTypes.labelled_equiv sensitivity_lat.
+Ltac case_leq l1 l2 := destruct (leq_dec Labels l1 l2) as [Hleq | Hnleq].
 
-
-
-Ltac case_leq l1 l2 := destruct (leq_dec sensitivity_lat l1 l2) as [?Hleq | ?Hnleq].
-
-Instance labelled_equit_equiv {Γ l} : Equivalence (labelled_equiv Γ l).
+Instance labelled_equit_equiv {Γ l} : Equivalence (labelled_equiv _ Γ l).
 Proof.
   constructor; unfold labelled_equiv.
-  - red. red. intros; auto.
-  - do 2 red. intros. symmetry; auto.
-  - do 2 red. intros. rewrite H; auto.
+  - red. auto.
+  - red. intros. symmetry; auto.
+  - red. intros. rewrite H; auto.
 Qed.
+
 Notation privacy_map := LabelledImp.privacy_map.
 Notation impExcE := LabelledImp.impExcE.
 Notation IOE := LabelledImp.IOE.
-Definition label_pi_eqit_secure_impstate  (b1 b2 : bool) (Γ : privacy_map sensitivity_lat) (l : label) {R1 R2 : Type} (RR : R1 -> R2 -> Prop )
-           (m1 : stateT (registers * map) (itree ((impExcE sensitivity_lat) +' (IOE sensitivity_lat))) R1) 
-           (m2 : stateT (registers * map ) (itree ((impExcE sensitivity_lat) +' (IOE sensitivity_lat))) R2) : Prop :=
-  forall σ1 σ2 regs1 regs2, labelled_equiv Γ l σ1 σ2 -> pi_eqit_secure _ (priv_exc_io sensitivity_lat) (product_rel (product_rel top2 (labelled_equiv Γ l)) RR) b1 b2 l (m1 (regs1,σ1)) (m2 (regs2, σ2)).
+Definition label_pi_eqit_secure_impstate  (b1 b2 : bool) (Γ : privacy_map Labels) (l : label) {R1 R2 : Type} (RR : R1 -> R2 -> Prop )
+           (m1 : stateT (registers * map) (itree ((impExcE Labels) +' (IOE Labels))) R1) 
+           (m2 : stateT (registers * map ) (itree ((impExcE Labels) +' (IOE Labels))) R2) : Prop :=
+  forall σ1 σ2 regs1 regs2, labelled_equiv _ Γ l σ1 σ2 -> pi_eqit_secure _ (priv_exc_io Labels) (product_rel (product_rel top2 (labelled_equiv _ Γ l)) RR) b1 b2 l (m1 (regs1,σ1)) (m2 (regs2, σ2)).
 
 Definition label_state_pi_sec_eutt {R1 R2} priv l (RR : R1 -> R2 -> Prop) m1 m2 :=
   label_pi_eqit_secure_impstate true true  priv l RR m1 m2.
 
-Definition sem_stmt (s : stmt) := interp_imp_inline (denote_stmt s).
+Definition sem_stmt (s : stmt _) := interp_imp_inline (denote_stmt _ s).
 
-Definition sem_throw_stmt (s : stmt) := interp_imp_inline (throw_prefix (denote_stmt s) ).
+Definition sem_throw_stmt (s : stmt _) := interp_imp_inline (throw_prefix (denote_stmt _ s) ).
 
-Definition sem_expr (e : expr) := LabelledImpInlineTypes.sem_expr e.
+Definition sem_expr (e : expr) := LabelledImpInlineTypes.sem_expr _ e.
 
 Definition state_equiv {E R} (m1 m2 : stateT map (itree E) R) := forall (σ : map), m1 σ ≈ m2 σ.
 
@@ -107,9 +105,9 @@ Proof.
     specialize (H σ1).  eapply proper_eutt_pi_secure_eutt; eauto.
 Qed.
 *)
-Context (Γ : privacy_map sensitivity_lat).
+Context (Γ : privacy_map Labels).
 
-Variant secure_stmt_at_label (observer pc lexn : label) (s : stmt) : Prop :=
+Variant secure_stmt_at_label (observer pc lexn : label) (s : stmt _) : Prop :=
   | ssal_leq : (leq pc observer) -> label_state_pi_sec_eutt Γ observer eq (sem_stmt s) (sem_stmt s) -> secure_stmt_at_label observer pc lexn s
   | ssal_nleq : (~ leq pc observer) -> label_state_pi_sec_eutt Γ observer top2 (sem_stmt s) (ret tt) -> secure_stmt_at_label observer pc lexn s.
 
@@ -148,7 +146,7 @@ Variant Rsense_unpriv (observer lexn : label) : unit + label -> Prop :=
   | rup_inl : Rsense_unpriv observer lexn (inl tt)
   | rup_priv_exc lpriv : ~ leq lpriv observer -> leq lpriv lexn -> Rsense_unpriv observer lexn (inr lpriv).
 
-Variant secure_throw_stmt_at_label (observer pc lexn : label) (s : stmt) : Prop :=
+Variant secure_throw_stmt_at_label (observer pc lexn : label) (s : stmt _) : Prop :=
   | stsal_leq : leq pc observer -> label_state_pi_sec_eutt Γ observer (Rsense observer lexn )
                                                        (sem_throw_stmt s) (sem_throw_stmt s) -> secure_throw_stmt_at_label observer pc lexn s
   | stsal_nleq : (~ leq pc observer) -> label_state_pi_sec_eutt Γ observer (fun sum _ => Rsense_unpriv observer lexn sum )
@@ -158,23 +156,23 @@ Variant secure_throw_stmt_at_label (observer pc lexn : label) (s : stmt) : Prop 
 Definition secure_throw_stmt pc lexn s := forall observer, secure_throw_stmt_at_label observer pc lexn s.
 
 Lemma pi_sem_stmt_ret_aux:
-  forall (s1 s2 : stmt ) (observer : label) (σ3 σ4 : map) (regs1 regs2 : registers),
+  forall (s1 s2 : stmt _) (observer : label) (σ3 σ4 : map) (regs1 regs2 : registers),
     (forall (σ1 σ2 : map) (regs1 regs2 : registers),
-        labelled_equiv Γ observer σ1 σ2 ->
-        pi_eqit_secure _ (priv_exc_io sensitivity_lat) (product_rel (product_rel top2 (labelled_equiv Γ observer)) top2)
+        labelled_equiv _ Γ observer σ1 σ2 ->
+        pi_eqit_secure _ (priv_exc_io _) (product_rel (product_rel top2 (labelled_equiv _ Γ observer)) top2)
                        true true observer (sem_stmt s1 (regs1, σ1)) (Ret ((regs2, σ2, tt)))) ->
     (forall (σ1 σ2 : map) (regs1 regs2 : registers),
-        labelled_equiv Γ observer σ1 σ2 ->
-        pi_eqit_secure _ (priv_exc_io sensitivity_lat) (product_rel (product_rel top2 (labelled_equiv Γ observer)) top2)
+        labelled_equiv _ Γ observer σ1 σ2 ->
+        pi_eqit_secure _ (priv_exc_io _) (product_rel (product_rel top2 (labelled_equiv _ Γ observer)) top2)
                        true true observer (sem_stmt s2 (regs1, σ1)) (Ret (regs2, σ2, tt))) ->
-    labelled_equiv Γ observer σ3 σ4 ->
-    pi_eqit_secure _ (priv_exc_io sensitivity_lat) (product_rel (product_rel top2 (labelled_equiv Γ observer)) eq) true
-                   true observer (interp_imp_inline (denote_stmt s1) (regs1, σ3))
-                   (interp_imp_inline (denote_stmt s2) (regs2, σ4)) .
+    labelled_equiv _ Γ observer σ3 σ4 ->
+    pi_eqit_secure _ (priv_exc_io _) (product_rel (product_rel top2 (labelled_equiv _ Γ observer)) eq) true
+                   true observer (interp_imp_inline (denote_stmt _ s1) (regs1, σ3))
+                   (interp_imp_inline (denote_stmt _ s2) (regs2, σ4)) .
 Proof.
   intros s1 s2 observer σ3 σ4 ? ? Hσ Hs1 Hs2.
-  eapply pi_eqit_secure_RR_imp with (RR1 := rcompose  (product_rel (product_rel top2 (labelled_equiv Γ observer)) (@top2 unit unit)) 
-                                                      (Basics.flip (product_rel (product_rel top2 (labelled_equiv Γ observer)) top2))).
+  eapply pi_eqit_secure_RR_imp with (RR1 := rcompose  (product_rel (product_rel top2 (labelled_equiv _ Γ observer)) (@top2 unit unit)) 
+                                                      (Basics.flip (product_rel (product_rel top2 (labelled_equiv _ Γ observer)) top2))).
   { intros [ [ ? σ5] [] ] [ [ ? σ6] [] ] Hr. inv Hr. inv REL1. inv REL2. split; auto.
     destruct r2 as [ [? σ7] [] ]. split; auto. inv H1. inv H. cbn in *. etransitivity; eauto. symmetry. auto.
   }
@@ -183,28 +181,28 @@ Proof.
 Qed.
 
 Lemma pi_sem_throw_stmt_ret_aux:
-  forall (lexn: label) (s1 s2 : stmt) (observer : label) (σ3 σ4 : map) (regs3 regs4 : registers),
+  forall (lexn: label) (s1 s2 : stmt _) (observer : label) (σ3 σ4 : map) (regs3 regs4 : registers),
     (forall (σ1 σ2 : map) (regs1 regs2 : registers),
-        labelled_equiv Γ observer σ1 σ2 ->
-        pi_eqit_secure _ (priv_exc_io sensitivity_lat)
-                       (product_rel (product_rel top2 (labelled_equiv Γ observer))
+        labelled_equiv _ Γ observer σ1 σ2 ->
+        pi_eqit_secure _ (priv_exc_io _)
+                       (product_rel (product_rel top2 (labelled_equiv _ Γ observer))
                                     (fun (sum : unit + label) (_ : unit) => Rsense_unpriv observer lexn sum)) true true observer
                        (sem_throw_stmt s1 (regs1, σ1)) (Ret (regs2, σ2, tt))) ->
     (forall (σ1 σ2 : map) (regs1 regs2 : registers),
-        labelled_equiv Γ observer σ1 σ2 ->
-        pi_eqit_secure _ (priv_exc_io sensitivity_lat)
-                       (product_rel (product_rel top2 (labelled_equiv Γ observer))
+        labelled_equiv _ Γ observer σ1 σ2 ->
+        pi_eqit_secure _ (priv_exc_io _)
+                       (product_rel (product_rel top2 (labelled_equiv _ Γ observer))
                                     (fun (sum : unit + label) (_ : unit) => Rsense_unpriv observer lexn sum)) true true observer
                        (sem_throw_stmt s2 (regs1, σ1)) (Ret (regs2, σ2, tt))) ->
-    labelled_equiv Γ observer σ3 σ4 ->
-    pi_eqit_secure _ (priv_exc_io sensitivity_lat)
-                   (product_rel (product_rel top2 (labelled_equiv Γ observer)) (Rsense observer lexn)) true true
-                   observer (interp_imp_inline (throw_prefix (denote_stmt s1)) (regs3, σ3))
-                   (interp_imp_inline (throw_prefix (denote_stmt s2)) (regs4, σ4)).
+    labelled_equiv _ Γ observer σ3 σ4 ->
+    pi_eqit_secure _ (priv_exc_io _)
+                   (product_rel (product_rel top2 (labelled_equiv _ Γ observer)) (Rsense observer lexn)) true true
+                   observer (interp_imp_inline (throw_prefix (denote_stmt _ s1)) (regs3, σ3))
+                   (interp_imp_inline (throw_prefix (denote_stmt _ s2)) (regs4, σ4)).
 Proof.
   intros lexn s1 s2 observer σ3 σ4 regs3 regs4 Hs1 Hs2 Hσ.
   (*  *)
-  set (product_rel (product_rel (@top2 registers registers) (labelled_equiv Γ observer)) (fun (sum : unit + label) ( _ : unit) => Rsense_unpriv observer lexn sum ) ) as HR.
+  set (product_rel (product_rel (@top2 registers registers) (labelled_equiv _ Γ observer)) (fun (sum : unit + label) ( _ : unit) => Rsense_unpriv observer lexn sum ) ) as HR.
   eapply pi_eqit_secure_RR_imp with (RR1 := rcompose HR (Basics.flip HR) ).
   { unfold HR. intros [ [ ? σ5] r1] [ [ ? σ6] r2] Hr. inv Hr. inv REL1. inv REL2.
     inv H. inv H1. cbn in *. repeat (split; cbn; auto). etransitivity; eauto. symmetry. auto.
@@ -217,11 +215,11 @@ Qed.
 
 Lemma lower_lexn_sound lexn1 lexn2 t1 t2 observer :
   leq lexn1 lexn2 ->
-  pi_eqit_secure _ (priv_exc_io sensitivity_lat)
-                 (product_rel (product_rel (@top2 registers registers) (labelled_equiv Γ observer)) (Rsense observer lexn1)) true true
+  pi_eqit_secure _ (priv_exc_io _)
+                 (product_rel (product_rel (@top2 registers registers) (labelled_equiv _ Γ observer)) (Rsense observer lexn1)) true true
                  observer t1 t2 ->
-  pi_eqit_secure _ (priv_exc_io sensitivity_lat)
-                 (product_rel (product_rel (@top2 registers registers) (labelled_equiv Γ observer)) (Rsense observer lexn2)) true true
+  pi_eqit_secure _ (priv_exc_io _)
+                 (product_rel (product_rel (@top2 registers registers) (labelled_equiv _ Γ observer)) (Rsense observer lexn2)) true true
                  observer t1 t2.
 Proof.
   intros. eapply pi_eqit_secure_RR_imp; try apply H0.
@@ -238,11 +236,11 @@ Qed.
 
 Lemma lower_lexn_sound' lexn1 lexn2 t1 t2 observer :
   leq lexn1 lexn2 ->
-  pi_eqit_secure _ (priv_exc_io sensitivity_lat)
-                 (product_rel (product_rel (@top2 registers registers) (labelled_equiv Γ observer)) (fun (sum : unit + label) (_ : unit) => Rsense_unpriv observer lexn1 sum)) true true
+  pi_eqit_secure _ (priv_exc_io _)
+                 (product_rel (product_rel (@top2 registers registers) (labelled_equiv _ Γ observer)) (fun (sum : unit + label) (_ : unit) => Rsense_unpriv observer lexn1 sum)) true true
                  observer t1 t2 ->
-  pi_eqit_secure _ (priv_exc_io sensitivity_lat)
-                 (product_rel (product_rel (@top2 registers registers) (labelled_equiv Γ observer)) (fun (sum : unit + label) (_ : unit) => Rsense_unpriv observer lexn2 sum)) true true
+  pi_eqit_secure _ (priv_exc_io _)
+                 (product_rel (product_rel (@top2 registers registers) (labelled_equiv _ Γ observer)) (fun (sum : unit + label) (_ : unit) => Rsense_unpriv observer lexn2 sum)) true true
                  observer t1 t2.
 Proof.
   intros. eapply pi_eqit_secure_RR_imp; try apply H0.
@@ -256,7 +254,7 @@ Qed.
 
 Lemma seq_well_typed_correct pc lexn1 lexn2 s1 s2 :
   secure_stmt pc lexn1 s1 -> secure_stmt (join pc lexn1) lexn2 s2 ->
-  secure_stmt pc (join lexn1 lexn2) (Seq s1 s2).
+  secure_stmt pc (join lexn1 lexn2) (Seq _ s1 s2).
 Proof.
   intros Hs1 Hs2 observer.
   specialize (Hs1 observer). inv Hs1.
@@ -272,14 +270,15 @@ Proof.
     eapply pi_eqit_secure_bind; eauto.
     intros [ [ ? σ3] [] ] [ [ ? σ4] [] ] [ [ _ Hσ'] _ ].
     specialize (Hs2 observer). inv Hs2; eauto.
-    + exfalso. apply H. eapply leq_trans_lat; eauto; apply sensitivity_latlaws.
-      cbn. destruct pc; destruct lexn1; auto.
+    + exfalso. apply H. eapply leq_trans_lat; eauto; apply HLabels.
+      cbn. destruct HLabels. rewrite join_assoc. rewrite join_idempot.
+      reflexivity. constructor; auto.
     + cbn in H2. eauto.
 Qed.
 
 Lemma seq_well_typed_correct' pc lexn1 lexn2 s1 s2 :
   secure_throw_stmt pc lexn1 s1 -> secure_throw_stmt (join pc lexn1) lexn2 s2 ->
-  secure_throw_stmt pc (join lexn1 lexn2) (Seq s1 s2).
+  secure_throw_stmt pc (join lexn1 lexn2) (Seq _ s1 s2).
 Proof.
   intros Hs1 Hs2 observer.
   specialize (Hs1 observer). inv Hs1.
@@ -292,19 +291,22 @@ Proof.
       * cbn in *.
         eapply pi_eqit_secure_RR_imp; try eapply H2; eauto.
         intros. inv H3. inv H4. repeat (split; auto). inv H5.
-        constructor.  constructor; destruct l1; destruct l2; destruct lexn1; destruct lexn2; cbn in *; try discriminate; auto.
-        constructor. destruct lpriv; destruct lexn1; destruct lexn2; cbn in *; try discriminate; auto. auto.
-        constructor; auto. destruct lpriv; destruct lexn1; destruct lexn2; cbn in *; try discriminate; auto.
+        constructor. constructor. eapply leq_trans_lat; eauto. apply leq_join_r; eauto.
+        eapply leq_trans_lat; eauto. apply leq_join_r; eauto.
+        constructor. eapply leq_trans_lat; eauto. apply leq_join_r; eauto. auto.
+        constructor. eapply leq_trans_lat; eauto. apply leq_join_r; eauto. auto.
       * cbn in *. cbn.
         cbn in Hσ'.
-        eapply lower_lexn_sound. apply leq_join_r; auto. apply sensitivity_latlaws.
+        eapply lower_lexn_sound. apply leq_join_r; auto.
         eapply pi_sem_throw_stmt_ret_aux; eauto.
     + cbn in H3, H4. subst. cbn. setoid_rewrite interp_state_ret. apply pi_eqit_secure_ret.
-      repeat (split; auto); constructor; eapply leq_trans_lat; eauto; try apply sensitivity_latlaws;
-      cbn; destruct lexn1; destruct lexn2; auto.
+      repeat (split; auto).
+      constructor; eapply leq_trans_lat; eauto; apply leq_join_l; auto.
     + specialize (Hs2 observer). inv Hs2; eauto.
-      * exfalso. apply H2. eapply leq_trans_lat; eauto; try apply sensitivity_latlaws.
-        cbn. destruct pc; destruct lexn1; destruct observer; cbn in *; try discriminate; auto.
+      * exfalso. apply H2. eapply leq_trans_lat; eauto; try apply HLabels.
+        enough (leq lexn1 observer); auto. cbn in H7.
+        destruct HLabels. rewrite H7. reflexivity.
+        eapply leq_trans_lat; eauto. apply leq_join_r; auto.
       * cbn in H3, H4. subst. cbn. setoid_rewrite interp_state_ret. cbn.
         cbn in H6. do 2 red in H6.
         match goal with 
@@ -316,12 +318,11 @@ Proof.
         -- cbn in H4. subst. apply pi_eqit_secure_ret. repeat (split; auto).
            constructor; auto. eapply leq_trans_lat; eauto; try apply leq_join_l; auto; apply sensitivity_latlaws.
         -- cbn in H8. subst. apply pi_eqit_secure_ret. repeat (split; auto).
-           constructor; auto. eapply leq_trans_lat; eauto. apply sensitivity_latlaws. apply leq_join_r; auto.
-           apply sensitivity_latlaws.
-           eapply leq_trans_lat; eauto; try apply leq_join_l; auto; apply sensitivity_latlaws.
+           constructor; auto. eapply leq_trans_lat; eauto. apply leq_join_r; auto.
+           eapply leq_trans_lat; eauto; try apply leq_join_l; auto.
     + specialize (Hs2 observer). inv Hs2; eauto.
       * exfalso. apply H2. eapply leq_trans_lat; eauto; 
-        try eapply leq_trans_lat; eauto; try apply leq_join_r; auto; apply sensitivity_latlaws.
+        try eapply leq_trans_lat; eauto; try apply leq_join_r; auto.
       * cbn. cbn in H3, H4. subst. setoid_rewrite interp_state_ret. cbn.
         cbn in H6.
         match goal with
@@ -335,8 +336,8 @@ Proof.
            constructor; auto. eapply leq_trans_lat; eauto; try apply leq_join_l; auto; apply sensitivity_latlaws.
         -- cbn in H8. subst. apply pi_eqit_secure_ret. repeat (split; auto). symmetry. auto.
            constructor; eapply leq_trans_lat; eauto; try apply leq_join_l; auto;
-           try eapply leq_trans_lat; eauto; try eapply leq_join_r; auto; apply sensitivity_latlaws.
-           Unshelve. 2 : apply lexn1. destruct lexn1; destruct lexn2; cbn; auto.
+           try eapply leq_trans_lat; eauto; try eapply leq_join_r; auto. 
+           Unshelve. 2 : apply lexn1. apply leq_refl_lat. auto.
   - right; auto. intros σ1 σ2 regs1 regs2 Hσ. unfold sem_throw_stmt, interp_imp_inline, interp_asm.
     cbn. setoid_rewrite throw_prefix_bind. setoid_rewrite interp_state_bind.
     cbn in H0. rewrite <- bind_ret_r with (s := Ret (regs2, σ2, tt) ).
@@ -354,7 +355,7 @@ Hint Resolve sensitivity_latlaws.
 Lemma try_catch_well_typed_correct pc lexn1 lexn2 s1 s2 :
   secure_stmt pc lexn1 s1 -> secure_throw_stmt pc lexn1 s1 ->
   secure_stmt (join pc lexn1) lexn2 s2 ->
-  secure_stmt pc lexn2 (TryCatch s1 s2).
+  secure_stmt pc lexn2 (TryCatch _ s1 s2).
 Proof.
   intros Hs1 Hs1t Hs2 observer.
   specialize (Hs1 observer). specialize (Hs1t observer).
@@ -370,14 +371,14 @@ Proof.
       * exfalso. apply H4. eapply leq_trans_lat; eauto.
         eapply leq_trans_lat; auto. apply leq_join_r; auto. eauto.
       * apply pi_eqit_secure_sym. do 2 red in H8. cbn in H8.
-        apply pi_eqit_secure_RR_imp with (RR1 := product_rel (product_rel (@top2 registers registers) (labelled_equiv Γ observer)) top2).
+        apply pi_eqit_secure_RR_imp with (RR1 := product_rel (product_rel (@top2 registers registers) (labelled_equiv _ Γ observer)) top2).
         { intros [ [ ? ?] [] ] [ [ ? ?] [] ] [ [? ?] ? ] . repeat (split; auto). symmetry. auto. }
         cbn in H5, H6. subst. setoid_rewrite interp_state_ret. eapply H8. symmetry. auto.
     + specialize (Hs2 observer). inv Hs2. 
       * exfalso. apply H4. eapply leq_trans_lat; eauto.
         eapply leq_trans_lat; auto. apply leq_join_r; auto. eauto.
       * do 2 red in H8.
-        apply pi_eqit_secure_RR_imp with (RR1 := product_rel (product_rel top2 (labelled_equiv Γ observer)) top2).
+        apply pi_eqit_secure_RR_imp with (RR1 := product_rel (product_rel top2 (labelled_equiv _ Γ observer)) top2).
         { intros [ [ ? ?] [] ] [ [ ? ?] [] ] [ [? ?] ? ] . inv H9. repeat (split; auto). }
         cbn in H8. cbn in H5, H6. subst. setoid_rewrite interp_state_ret. eapply H8. auto. 
   - right; auto. unfold sem_stmt, interp_imp_inline, interp_asm. do 2 red. intros σ1 σ2 regs1 regs2 Hσ.
@@ -398,7 +399,7 @@ Qed.
 Lemma try_catch_well_typed_correct' pc lexn1 lexn2 s1 s2 :
   secure_stmt pc lexn1 s1 -> secure_throw_stmt pc lexn1 s1 ->
   secure_throw_stmt (join pc lexn1) lexn2 s2 ->
-  secure_throw_stmt pc lexn2 (TryCatch s1 s2).
+  secure_throw_stmt pc lexn2 (TryCatch _ s1 s2).
 Proof.
   intros Hs1 Hs1t Hs2 observer. specialize (Hs1 observer).
   specialize (Hs1t observer). inv Hs1; inv Hs1t; try contradiction.
@@ -465,22 +466,22 @@ Proof.
 Qed.
 
 Lemma pi_eqit_secure_while_ret_aux:
-  forall (e : expr) (s : stmt) (observer : label),
+  forall (e : expr) (s : stmt _) (observer : label),
     label_state_pi_sec_eutt Γ observer top2 (sem_stmt s) (ret tt) ->
     forall (σ1 σ2 : map) (regs1 regs2 : registers),
-      labelled_equiv Γ observer σ1 σ2 ->
-      pi_eqit_secure _ (priv_exc_io sensitivity_lat)
-                     (product_rel (product_rel top2 (labelled_equiv Γ observer)) top2) true true
-                     observer (sem_stmt (While e s) (regs1, σ1)) (Ret (regs2, σ2, tt)).
+      labelled_equiv _ Γ observer σ1 σ2 ->
+      pi_eqit_secure _ (priv_exc_io _)
+                     (product_rel (product_rel top2 (labelled_equiv _ Γ observer)) top2) true true
+                     observer (sem_stmt (While _ e s) (regs1, σ1)) (Ret (regs2, σ2, tt)).
 Proof.
   intros e s observer H0 σ1 σ2 regs1 regs2 H3.
   unfold sem_stmt, interp_imp_inline, interp_asm.
   cbn. specialize (@interp_state_iter') as Hisi. red in Hisi. setoid_rewrite Hisi.
-  eapply pi_eqit_secure_iter_ret with (Rinv := product_rel (product_rel top2 (labelled_equiv Γ observer)) eq ).
+  eapply pi_eqit_secure_iter_ret with (Rinv := product_rel (product_rel top2 (labelled_equiv _ Γ observer)) eq ).
   2 : repeat (split; auto).
   intros [ [ ? σ3] [] ] [ [ _ Hσ3] _ ]. cbn.
   setoid_rewrite interp_state_bind. rewrite bind_bind.
-  specialize (expr_only_ret' e (r, σ3)) as [n Hn]. setoid_rewrite Hn.
+  specialize (expr_only_ret'  _ e (r, σ3)) as [n Hn]. setoid_rewrite Hn.
   rewrite bind_ret_l. destruct n.
   + cbn. rewrite interp_state_ret, bind_ret_l. cbn. apply pi_eqit_secure_ret.
     constructor. repeat (split; auto).
@@ -493,26 +494,26 @@ Proof.
 Qed.
 
 Lemma pi_eqit_secure_while_ret_throw_aux:
-  forall (e : expr) (s : stmt) (observer lexn : label),
+  forall (e : expr) (s : stmt _) (observer lexn : label),
     label_state_pi_sec_eutt Γ observer (fun (sum : unit + label) (_ : unit) => Rsense_unpriv observer lexn sum)
                             (sem_throw_stmt s) (ret tt) ->
     forall (σ1 σ2 : map) (regs1 regs2 : registers),
-      labelled_equiv Γ observer σ1 σ2 -> 
-      pi_eqit_secure _ (priv_exc_io sensitivity_lat)
-                     (product_rel (product_rel top2 (labelled_equiv Γ observer))
+      labelled_equiv _ Γ observer σ1 σ2 -> 
+      pi_eqit_secure _ (priv_exc_io _)
+                     (product_rel (product_rel top2 (labelled_equiv _ Γ observer))
                                   (fun (sum : unit + label) (_ : unit) => Rsense_unpriv observer lexn sum)) true true observer
-                     (sem_throw_stmt (While e s) (regs1, σ1)) (Ret (regs2, σ2, tt)).
+                     (sem_throw_stmt (While _ e s) (regs1, σ1)) (Ret (regs2, σ2, tt)).
 Proof.
   intros e s observer lexn H0 σ1 σ2 regs1 regs2 Hσ.
   unfold sem_throw_stmt, interp_imp_inline, interp_asm.
   cbn. setoid_rewrite throw_prefix_iter.
   specialize (@interp_state_iter') as Hisi. red in Hisi. setoid_rewrite Hisi.
-  apply pi_eqit_secure_iter_ret with (Rinv := product_rel (product_rel top2 (labelled_equiv Γ observer)) eq).
+  apply pi_eqit_secure_iter_ret with (Rinv := product_rel (product_rel top2 (labelled_equiv _ Γ observer)) eq).
   2 : repeat (split; auto).
   intros [ [ ? σ3] [] ] [ [ _ Hσ3] _ ]. cbn. cbn in Hσ3. setoid_rewrite throw_prefix_bind.
   repeat setoid_rewrite interp_state_bind. repeat rewrite bind_bind.
   rewrite throw_prefix_denote_expr. rewrite interp_state_bind, bind_bind.
-  specialize (expr_only_ret' e (r, σ3)) as [n Hn]. 
+  specialize (expr_only_ret' _ e (r, σ3)) as [n Hn]. 
   setoid_rewrite Hn.
   rewrite bind_ret_l, interp_state_ret, bind_ret_l. cbn.
   destruct n.
@@ -532,7 +533,7 @@ Proof.
 Qed.
 
 Lemma while_well_typed_correct e le pc lexn s :
-  secure_expr le e -> secure_stmt (join pc (join le lexn)) lexn s -> secure_stmt pc lexn (While e s).
+  secure_expr le e -> secure_stmt (join pc (join le lexn)) lexn s -> secure_stmt pc lexn (While _ e s).
 Proof.
   intros He Hs observer.
   specialize (He observer). specialize (Hs observer).
@@ -540,7 +541,7 @@ Proof.
   - left. eapply leq_trans_lat; try apply H; auto. apply leq_join_l; auto.
     do 2 red. intros σ1 σ2 regs1 regs2 Hσ. unfold sem_stmt, interp_imp_inline, interp_asm. cbn.
     specialize (@interp_state_iter') as Hisi. red in Hisi. setoid_rewrite Hisi.
-    apply secure_eqit_iter with (RA := product_rel (product_rel top2 (labelled_equiv Γ observer)) eq );
+    apply secure_eqit_iter with (RA := product_rel (product_rel top2 (labelled_equiv _ Γ observer)) eq );
       auto.
     clear σ1 σ2 Hσ. intros [ [ ? σ1] [] ] [ [ ? σ2] [] ] [ [ _ Hσ] _ ].
     cbn. setoid_rewrite interp_state_bind. repeat rewrite bind_bind.
@@ -556,7 +557,7 @@ Proof.
       constructor; repeat (split; auto).
     + repeat (split; auto).
   - exfalso. apply H1.
-    eapply leq_trans_lat with (l2 := join_sense le lexn); eauto. 
+    eapply leq_trans_lat with (l2 := join le lexn); eauto. 
     apply leq_join_l; auto.
     eapply leq_trans_lat; try apply leq_join_r; auto. eauto.
   - case_leq pc observer.
@@ -574,7 +575,7 @@ Qed.
 
 
 Lemma while_well_typed_correct' e le pc lexn s : 
-  secure_expr le e -> secure_throw_stmt (join pc (join le lexn)) lexn s -> secure_throw_stmt pc lexn (While e s).
+  secure_expr le e -> secure_throw_stmt (join pc (join le lexn)) lexn s -> secure_throw_stmt pc lexn (While _ e s).
 Proof.
   intros He Hs observer.
   specialize (He observer). specialize (Hs observer).
@@ -583,7 +584,7 @@ Proof.
     do 2 red. intros σ1 σ2 regs1 regs2 Hσ. unfold sem_throw_stmt, interp_imp_inline, interp_asm. cbn.
     setoid_rewrite throw_prefix_iter.
     specialize (@interp_state_iter') as Hisi. red in Hisi. setoid_rewrite Hisi.
-    eapply secure_eqit_iter with (RA := product_rel (product_rel top2 (labelled_equiv Γ observer)) eq ); auto.
+    eapply secure_eqit_iter with (RA := product_rel (product_rel top2 (labelled_equiv _ Γ observer)) eq ); auto.
     intros [ [ ? σ3] [] ] [ [ ? σ4] [] ] [ [ _ Hσ'] _ ]. cbn. setoid_rewrite throw_prefix_bind.
     repeat setoid_rewrite interp_state_bind. repeat rewrite bind_bind.
     setoid_rewrite throw_prefix_denote_expr. setoid_rewrite interp_state_bind.
@@ -604,16 +605,16 @@ Proof.
       * exfalso. apply H4.
         eapply leq_trans_lat; eauto.
         eapply leq_trans_lat; try apply H; auto.
-        eapply leq_trans_lat with (l2 := join_sense le lexn); eauto.
+        eapply leq_trans_lat with (l2 := join le lexn); eauto.
         apply leq_join_r; auto. apply leq_join_r; auto.
       * exfalso.  apply H4.
         eapply leq_trans_lat; eauto.
         eapply leq_trans_lat; try apply H; auto.
-        eapply leq_trans_lat with (l2 := join_sense le lexn); eauto.
+        eapply leq_trans_lat with (l2 := join le lexn); eauto.
         apply leq_join_r; auto. apply leq_join_r; auto.
     + repeat (split; auto).
   - exfalso. apply H1. eapply leq_trans_lat; eauto. 
-    eapply leq_trans_lat with (l2 := join_sense le lexn); auto.  
+    eapply leq_trans_lat with (l2 := join le lexn); auto.  
     apply leq_join_l; auto. apply leq_join_r; auto.
   - case_leq pc observer.
     + left; auto. intros σ1 σ2 regs1 regs2 Hσ.
@@ -632,13 +633,13 @@ Qed.
 Lemma if_well_typed_correct e le pc lexn1 lexn2 s1 s2 :
   secure_expr le e -> secure_stmt (join pc le) lexn1 s1 ->
   secure_stmt (join pc le) lexn2 s2 ->
-  secure_stmt pc (join lexn1 lexn2) (If e s1 s2).
+  secure_stmt pc (join lexn1 lexn2) (If _ e s1 s2).
 Proof.
   intros He Hs1 Hs2 observer.
   specialize (Hs1 observer). specialize (Hs2 observer).
   specialize (He observer).
   inv Hs1; inv Hs2; inv He; try contradiction.
-  - left; auto. eapply leq_trans_lat with (l2 := join_sense pc le);  eauto.
+  - left; auto. eapply leq_trans_lat with (l2 := join pc le);  eauto.
     apply leq_join_l; auto.
     intros σ1 σ2 regs1 regs2 Hσ. unfold sem_stmt, interp_imp_inline, interp_asm.
     cbn. setoid_rewrite interp_state_bind.
@@ -650,33 +651,33 @@ Proof.
   - right. intro. apply H. apply leq_join_lub; auto.
     intros σ1 σ2 regs1 regs2 Hσ. unfold sem_stmt, interp_imp_inline. cbn.
     setoid_rewrite interp_state_bind.
-    specialize (expr_only_ret' e (regs1, σ1)) as [n Hn]. setoid_rewrite Hn.
+    specialize (expr_only_ret' _ e (regs1, σ1)) as [n Hn]. setoid_rewrite Hn.
     rewrite bind_ret_l. destruct n; cbn in *; eauto.
   - case_leq pc observer.
     + left; auto. intros σ1 σ2 regs1 regs2 Hσ. unfold sem_stmt, interp_imp_inline. cbn.
       setoid_rewrite interp_state_bind.
-      specialize (expr_only_ret' e (regs1, σ1)) as [n1 Hn1]. setoid_rewrite Hn1.
-      specialize (expr_only_ret' e (regs2, σ2)) as [n2 Hn2]. setoid_rewrite Hn2.
+      specialize (expr_only_ret' _ e (regs1, σ1)) as [n1 Hn1]. setoid_rewrite Hn1.
+      specialize (expr_only_ret' _ e (regs2, σ2)) as [n2 Hn2]. setoid_rewrite Hn2.
       setoid_rewrite bind_ret_l.
       destruct n1; destruct n2; cbn;
         eapply pi_sem_stmt_ret_aux; eauto.
     + right; auto.
       intros σ1 σ2 regs1 regs2 Hσ. unfold sem_stmt, interp_imp_inline, interp_asm. cbn.
       setoid_rewrite interp_state_bind.
-      specialize (expr_only_ret' e (regs1, σ1)) as [n1 Hn1]. setoid_rewrite Hn1.
+      specialize (expr_only_ret' _ e (regs1, σ1)) as [n1 Hn1]. setoid_rewrite Hn1.
       rewrite bind_ret_l. destruct n1; cbn in *; eauto.
 Qed.
 
 Lemma if_well_typed_correct' e le pc lexn1 lexn2 s1 s2 :
   secure_expr le e -> secure_throw_stmt (join pc le) lexn1 s1 ->
   secure_throw_stmt (join pc le) lexn2 s2 ->
-  secure_throw_stmt pc (join lexn1 lexn2) (If e s1 s2).
+  secure_throw_stmt pc (join lexn1 lexn2) (If _ e s1 s2).
 Proof.
   intros He Hs1 Hs2 observer.
   specialize (Hs1 observer). specialize (Hs2 observer).
   specialize (He observer).
   inv Hs1; inv Hs2; inv He; try contradiction.
-  - left; auto. eapply leq_trans_lat with (l2 := join_sense pc le);  eauto.
+  - left; auto. eapply leq_trans_lat with (l2 := join pc le);  eauto.
     apply leq_join_l; auto.
     unfold sem_throw_stmt, interp_imp_inline, interp_asm. intros σ1 σ2 regs1 regs2 Hσ.
     cbn. setoid_rewrite throw_prefix_bind.
@@ -696,7 +697,7 @@ Proof.
     cbn. setoid_rewrite throw_prefix_bind.
     setoid_rewrite throw_prefix_denote_expr.
     repeat rewrite interp_state_bind. repeat rewrite bind_bind.
-    specialize (expr_only_ret' e (regs1, σ1)) as [n1 Hn1]. setoid_rewrite Hn1.
+    specialize (expr_only_ret' _ e (regs1, σ1)) as [n1 Hn1]. setoid_rewrite Hn1.
     rewrite bind_ret_l. rewrite interp_state_ret, bind_ret_l.
     cbn.
     destruct n1; cbn in *; eapply lower_lexn_sound'; eauto.
@@ -706,8 +707,8 @@ Proof.
       cbn. setoid_rewrite throw_prefix_bind. setoid_rewrite interp_state_bind.
       setoid_rewrite throw_prefix_denote_expr. setoid_rewrite interp_state_bind.
       repeat rewrite bind_bind. 
-      specialize (expr_only_ret' e (regs1, σ1)) as [n1 Hn1]. setoid_rewrite Hn1.
-      specialize (expr_only_ret' e (regs2, σ2)) as [n2 Hn2]. setoid_rewrite Hn2.
+      specialize (expr_only_ret' _ e (regs1, σ1)) as [n1 Hn1]. setoid_rewrite Hn1.
+      specialize (expr_only_ret' _ e (regs2, σ2)) as [n2 Hn2]. setoid_rewrite Hn2.
       setoid_rewrite bind_ret_l. setoid_rewrite interp_state_ret.
       setoid_rewrite bind_ret_l. cbn. 
       assert (label_state_pi_sec_eutt Γ observer
@@ -723,10 +724,14 @@ Proof.
      intros σ1 σ2 regs1 regs2 Hσ. unfold sem_throw_stmt, interp_imp_inline, interp_asm. cbn.
      setoid_rewrite throw_prefix_bind. setoid_rewrite throw_prefix_denote_expr.
      repeat rewrite interp_state_bind. repeat rewrite bind_bind.
-     specialize (expr_only_ret' e (regs1, σ1)) as [n1 Hn1]. setoid_rewrite Hn1.
+     specialize (expr_only_ret' _ e (regs1, σ1)) as [n1 Hn1]. setoid_rewrite Hn1.
      rewrite bind_ret_l. rewrite interp_state_ret, bind_ret_l. cbn.
      destruct n1; try eapply lower_lexn_sound'; cbn in *; eauto.
-     destruct lexn1; destruct lexn2; auto. destruct lexn1; destruct lexn2; auto.
+     destruct HLabels.
+     rewrite join_comm. rewrite <- join_assoc. rewrite join_idempot. reflexivity.
+     constructor; auto.
+     destruct HLabels. rewrite join_assoc. rewrite join_idempot. reflexivity.
+     constructor; auto.
 Qed.
 
 Lemma secure_expr_upward_close
@@ -739,7 +744,7 @@ Proof.
     + left; auto.
     + right; auto.
       exists 0. do 2 red. intros. cbn.
-      specialize (expr_only_ret' e (regs1, σ1)) as [n Hn]. rewrite Hn.
+      specialize (expr_only_ret' _ e (regs1, σ1)) as [n Hn]. rewrite Hn.
       apply pi_eqit_secure_ret. repeat (split; auto).
   - case_leq l2 observer.
     + left; auto. exfalso. apply H. eapply leq_trans_lat; eauto.
@@ -748,7 +753,7 @@ Qed.
 
 Lemma assign_well_typed_correct e le pc x : 
   secure_expr le e -> leq (join le pc) (Γ x) ->
-  secure_stmt pc bot (Assign x e).
+  secure_stmt pc bot (Assign _ x e).
 Proof.
   intros Hle Hx. 
   assert (Hpc : leq pc (Γ x) ).
@@ -770,8 +775,8 @@ Proof.
     + left; auto. 
       destruct H0 as [n Hn]. unfold sem_stmt.
       cbn. unfold interp_imp_inline, interp_asm. do 2 red. intros. setoid_rewrite interp_state_bind.
-      specialize (expr_only_ret' e (regs1, σ1)) as [n1 Hn1]. setoid_rewrite Hn1.
-      specialize (expr_only_ret' e (regs2, σ2)) as [n2 Hn2]. setoid_rewrite Hn2.
+      specialize (expr_only_ret' _ e (regs1, σ1)) as [n1 Hn1]. setoid_rewrite Hn1.
+      specialize (expr_only_ret' _ e (regs2, σ2)) as [n2 Hn2]. setoid_rewrite Hn2.
       setoid_rewrite bind_ret_l. cbn. setoid_rewrite interp_state_trigger.
       cbn. apply pi_eqit_secure_ret. repeat (split; auto).
       cbn. apply update_labelled_equiv_invisible; auto. symmetry.
@@ -779,7 +784,7 @@ Proof.
     + right; auto.
       unfold sem_stmt, interp_imp_inline, interp_asm. cbn. intros σ1 σ2 regs1 regs2 Hσ.
       setoid_rewrite interp_state_bind.
-      specialize (expr_only_ret' e (regs1, σ1)) as [n1 Hn1]. setoid_rewrite Hn1.
+      specialize (expr_only_ret' _ e (regs1, σ1)) as [n1 Hn1]. setoid_rewrite Hn1.
       rewrite bind_ret_l. setoid_rewrite interp_state_trigger.
       cbn. apply pi_eqit_secure_ret. repeat (split; auto).
       cbn. apply update_labelled_equiv_invisible; auto.
@@ -787,7 +792,7 @@ Qed.
 
 Lemma assign_well_typed_correct' e le pc x : 
   secure_expr le e -> leq (join le pc) (Γ x) ->
-  secure_throw_stmt pc bot (Assign x e).
+  secure_throw_stmt pc bot (Assign _ x e).
 Proof.
   intros Hle Hx. 
   assert (Hpc : leq pc (Γ x) ).
@@ -819,8 +824,8 @@ Proof.
       cbn. unfold interp_imp_inline, interp_asm. do 2 red. intros. 
       setoid_rewrite throw_prefix_bind. setoid_rewrite throw_prefix_denote_expr.
       repeat setoid_rewrite interp_state_bind.
-      specialize (expr_only_ret' e (regs1, σ1)) as [n1 Hn1]. setoid_rewrite Hn1.
-      specialize (expr_only_ret' e (regs2, σ2)) as [n2 Hn2]. setoid_rewrite Hn2.
+      specialize (expr_only_ret' _ e (regs1, σ1)) as [n1 Hn1]. setoid_rewrite Hn1.
+      specialize (expr_only_ret' _ e (regs2, σ2)) as [n2 Hn2]. setoid_rewrite Hn2.
       repeat rewrite bind_ret_l. tau_steps.
       apply pi_eqit_secure_ret. repeat (split; auto).
       cbn. apply update_labelled_equiv_invisible; auto. symmetry.
@@ -831,7 +836,7 @@ Proof.
       setoid_rewrite throw_prefix_bind. 
       setoid_rewrite interp_state_bind. rewrite throw_prefix_denote_expr.
       setoid_rewrite interp_state_bind.
-      specialize (expr_only_ret' e (regs1, σ1)) as [n1 Hn1]. setoid_rewrite Hn1.
+      specialize (expr_only_ret' _ e (regs1, σ1)) as [n1 Hn1]. setoid_rewrite Hn1.
       tau_steps.
       apply pi_eqit_secure_ret.
       repeat (split; auto). 2 : constructor. cbn. apply update_labelled_equiv_invisible; auto.
@@ -840,7 +845,7 @@ Qed.
 
 Lemma print_well_typed_correct pc le lp e :
   secure_expr le e -> leq (join le pc) lp ->
-  secure_stmt pc bot (Output lp e).
+  secure_stmt pc bot (Output _ lp e).
 Proof.
   intros He0 Hle1.
   assert (Hle : leq le lp).
@@ -862,14 +867,14 @@ Proof.
   - case_leq pc observer.
     + left; auto. unfold sem_stmt, interp_imp_inline, interp_asm. intros σ1 σ2 regs1 regs2 Hσ.
       cbn. setoid_rewrite interp_state_bind.
-      specialize (expr_only_ret' e (regs1, σ1)) as [n1 Hn1]. setoid_rewrite Hn1.
-      specialize (expr_only_ret' e (regs2, σ2)) as [n2 Hn2]. setoid_rewrite Hn2.
+      specialize (expr_only_ret' _ e (regs1, σ1)) as [n1 Hn1]. setoid_rewrite Hn1.
+      specialize (expr_only_ret' _ e (regs2, σ2)) as [n2 Hn2]. setoid_rewrite Hn2.
       setoid_rewrite bind_ret_l. setoid_rewrite interp_state_trigger.
       cbn. setoid_rewrite bind_trigger. apply pi_eqit_secure_priv_vislr; auto.
       intros [] []. apply pi_eqit_secure_ret. repeat (split; auto).
     + right; auto. unfold sem_stmt, interp_imp_inline, interp_asm. intros σ1 σ2 regs1 regs2 Hσ.
       cbn. setoid_rewrite interp_state_bind.
-      specialize (expr_only_ret' e (regs1, σ1)) as [n1 Hn1]. setoid_rewrite Hn1.
+      specialize (expr_only_ret' _ e (regs1, σ1)) as [n1 Hn1]. setoid_rewrite Hn1.
       rewrite bind_ret_l. rewrite interp_state_trigger. cbn. rewrite bind_trigger.
       apply pi_eqit_secure_priv_visl; auto. intros [].
       apply pi_eqit_secure_ret. repeat (split; auto).
@@ -877,7 +882,7 @@ Qed.
 
 Lemma print_well_typed_correct' pc le lp e :
   secure_expr le e -> leq (join le pc) lp ->
-  secure_throw_stmt pc bot (Output lp e).
+  secure_throw_stmt pc bot (Output _ lp e).
 Proof.
   intros He0 Hle1.
   assert (Hle : leq le lp).
@@ -907,8 +912,8 @@ Proof.
       setoid_rewrite throw_prefix_denote_expr. 
       repeat setoid_rewrite interp_state_bind.
       repeat rewrite bind_bind.
-      specialize (expr_only_ret' e (regs1, σ1)) as [n1 Hn1]. setoid_rewrite Hn1.
-      specialize (expr_only_ret' e (regs2, σ2)) as [n2 Hn2]. setoid_rewrite Hn2.
+      specialize (expr_only_ret' _ e (regs1, σ1)) as [n1 Hn1]. setoid_rewrite Hn1.
+      specialize (expr_only_ret' _ e (regs2, σ2)) as [n2 Hn2]. setoid_rewrite Hn2.
       setoid_rewrite bind_ret_l.
       setoid_rewrite interp_state_ret. setoid_rewrite bind_ret_l. cbn.
       setoid_rewrite throw_prefix_ev.
@@ -922,7 +927,7 @@ Proof.
       setoid_rewrite throw_prefix_bind. setoid_rewrite interp_state_bind.
       setoid_rewrite throw_prefix_denote_expr.
       setoid_rewrite interp_state_bind.
-      specialize (expr_only_ret' e (regs1, σ1)) as [n1 Hn1]. setoid_rewrite Hn1.
+      specialize (expr_only_ret' _ e (regs1, σ1)) as [n1 Hn1]. setoid_rewrite Hn1.
       repeat rewrite bind_ret_l. 
       rewrite interp_state_ret. rewrite bind_ret_l. cbn.
       setoid_rewrite throw_prefix_ev.
@@ -934,7 +939,7 @@ Proof.
 Qed.
 
 Lemma skip_well_typed_correct pc :
-  secure_stmt pc bot Skip.
+  secure_stmt pc bot (Skip _).
 Proof.
   intros observer. case_leq pc observer.
   - left; auto. do 2 red. unfold sem_stmt. intros σ1 σ2 regs1 regs2 Hσ.
@@ -946,7 +951,7 @@ Proof.
 Qed.
 
 Lemma skip_well_typed_correct' pc :
-  secure_throw_stmt pc bot Skip.
+  secure_throw_stmt pc bot (Skip _).
 Proof.
   intros observer. case_leq pc observer.
   - left; auto. do 2 red. unfold sem_throw_stmt. intros σ1 σ2 regs1 regs2 Hσ.
@@ -960,12 +965,13 @@ Proof.
 Qed.
 
 Lemma raise_well_typed pc lexn :
-  leq pc lexn -> secure_stmt pc lexn (Raise lexn).
+  leq pc lexn -> secure_stmt pc lexn (Raise _ lexn).
 Proof.
   intros Hpc observer. case_leq pc observer.
   - left; auto. unfold sem_stmt, interp_imp. do 2 red. intros.
     cbn. setoid_rewrite bind_trigger. setoid_rewrite interp_state_vis.
     cbn. setoid_rewrite bind_trigger. setoid_rewrite bind_vis.
+    rename Hleq into Hleq'.
     case_leq lexn observer.
     + apply pi_eqit_secure_pub_vis. auto. intros [].
     + apply pi_eqit_secure_priv_vislr; auto. intros [].
@@ -977,7 +983,7 @@ Proof.
 Qed.
 
 Lemma raise_well_typed' pc lexn :
-  leq pc lexn -> secure_throw_stmt pc lexn (Raise lexn).
+  leq pc lexn -> secure_throw_stmt pc lexn (Raise _ lexn).
 Proof.
   intros Hpc observer. case_leq pc observer.
   - left; auto. unfold sem_throw_stmt, interp_imp_inline, interp_asm.
@@ -994,27 +1000,27 @@ Proof.
     apply Hnleq. eapply leq_trans_lat; eauto.
 Qed.
 
-Definition well_typed_expr := LabelledImpInlineTypes.well_typed_expr Γ.
+Definition well_typed_expr := LabelledImpInlineTypes.well_typed_expr _ Γ.
 
 
 (* rework this definition to have only public exceptions*)
-Inductive well_typed_stmt : label -> label -> stmt -> Prop :=
+Inductive well_typed_stmt : label -> label -> stmt _ -> Prop :=
   | wts_manual pc lexn s : secure_stmt pc lexn s /\ secure_throw_stmt pc lexn s /\ valid_stmt s -> 
                            well_typed_stmt pc lexn s
-  | wts_skip pc : well_typed_stmt pc bot Skip
+  | wts_skip pc : well_typed_stmt pc bot (Skip _)
   | wts_seq pc lexn1 lexn2 s1 s2 : well_typed_stmt pc lexn1 s1 -> well_typed_stmt (join pc lexn1) lexn2 s2 ->
-                                   well_typed_stmt pc (join lexn1 lexn2) (Seq s1 s2)
+                                   well_typed_stmt pc (join lexn1 lexn2) (Seq _ s1 s2)
   | wts_assign pc l x e : well_typed_expr l e -> leq (join l pc) (Γ x) ->
-                          well_typed_stmt pc bot (Assign x e)
+                          well_typed_stmt pc bot (Assign _ x e)
   | wts_print pc le lp e : well_typed_expr le e -> leq (join le pc) lp ->
-                           well_typed_stmt pc bot (Output lp e)
+                           well_typed_stmt pc bot (Output _ lp e)
   | wts_if pc le e lexn1 lexn2 s1 s2 : well_typed_expr le e -> well_typed_stmt (join pc le) lexn1 s1 -> well_typed_stmt (join pc le) lexn2 s2 ->
-                                       well_typed_stmt pc (join lexn1 lexn2) (If e s1 s2)
+                                       well_typed_stmt pc (join lexn1 lexn2) (If _ e s1 s2)
   | wts_while e le pc lexn s : well_typed_expr le e -> well_typed_stmt (join pc (join le lexn)) lexn s ->
-                         well_typed_stmt pc lexn (While e s)
-  | wts_raise pc lexn : leq pc lexn -> well_typed_stmt pc lexn (Raise lexn)
+                         well_typed_stmt pc lexn (While _ e s)
+  | wts_raise pc lexn : leq pc lexn -> well_typed_stmt pc lexn (Raise _ lexn)
   | wts_try pc lexn1 lexn2 s1 s2 : well_typed_stmt pc lexn1 s1 -> well_typed_stmt (join pc lexn1) lexn2 s2 ->
-                                   well_typed_stmt pc lexn2 (TryCatch s1 s2)
+                                   well_typed_stmt pc lexn2 (TryCatch _ s1 s2)
 .
 
 Lemma well_typed_expr_correct e l : 
@@ -1061,7 +1067,7 @@ Proof.
 Qed.
 
 Lemma secure_stmt_lower_pc:
-  forall (pc2 : label) lexn (s : stmt),
+  forall (pc2 : label) lexn (s : stmt _ ),
     secure_stmt pc2 lexn s -> forall pc1 : L, leq pc1 pc2 -> secure_stmt pc1 lexn s.
 Proof.
   intros pc2 lexn s H pc1 Hpc observer.
@@ -1074,7 +1080,7 @@ Proof.
 Qed.
 
 Lemma secure_throw_stmt_lower_pc:
-  forall (pc lexn : label) (s : stmt),
+  forall (pc lexn : label) (s : stmt _),
     secure_throw_stmt pc lexn s -> forall pc1 : L, leq pc1 pc -> secure_throw_stmt pc1 lexn s.
 Proof.
   intros pc lexn s H pc1 Hpc observer.
